more work on varint encode function

Varint.fst
@@ -9,6 +9,7 @@ open FStar.Int.Cast.Full
 open FStar.Seq
 open FStar.List.Tot
 
+module U = FStar.UInt
 module U8 = FStar.UInt8
 module U16 = FStar.UInt16
 module U32 = FStar.UInt32
@@ -20,19 +21,43 @@ module List = FStar.List.Tot
 let rec valid (v:list UInt8.t) : bool = 
   match v with 
   | [] -> false
-    (* A one-byte varint is valid if the continuation bit is zero *)
-  | msb :: [] -> U8.(msb &^ 128uy) = 0uy
+    (* A one-byte varint is valid if the continuation bit is zero,
+       which is equivalent to the number fitting into 7 bits *)
+  | msb :: [] -> UInt.fits (U8.v msb) 7
     (* Otherwise the continuation bit should be one *)
   | msb :: rest -> (U8.(msb &^ 0x80uy) = 128uy) && valid rest
 
-let varint = v:list UInt8.t{length v >= 1 /\ length v <= 10 /\ valid v}
+let varint = v:list UInt8.t{length v >= 1 /\ valid v}
 
 
-let encode (x: UInt64.t) : varint = 
-  assert UInt.logand_le (U64.v x) 0x7F;
+// let rec encode (l:pos{l % 8 = 0}) (x: U.uint_t l) : Tot varint (decreases l) = 
+//   assert l > 7; 
+//   let nextByte = U.logand x (U.to_uint_t l 0x7F) in 
+//   let rest = U.(shift_right x 7) in
+//   UInt.logand_le x (U.to_uint_t l 0x7F);
+//   assert nextByte < 128;
+//   assert U.fits nextByte 8;
+//   if rest = U.zero l then
+//     [U8.uint_to_t nextByte]
+//   else 
+//     let nextByte = U8.(uint_to_t nextByte |^ 128uy) in 
+//     [nextByte]
+
+let rec encode (x: U64.t) : Tot varint (decreases (U64.v x)) = 
   let nextByte = Cast.uint64_to_uint8 (U64.logand x 0x7FuL) in 
   let rest = U64.(x >>^ 7ul) in
-  [nextByte] 
+  UInt.logand_le (U64.v x) 0x7F;
+  assert UInt.fits U8.(v nextByte) 7;
+  if rest = 0uL then 
+    [nextByte]
+  else 
+    let nextByte = U8.(nextByte |^ 128uy) in
+    assume U64.v rest < U64.v x;
+    let restEnc = encode rest in
+    assert valid restEnc;
+    assume U8.(nextByte &^ 0x80uy) = 128uy;
+    List.append [nextByte] restEnc
+  
 
 let rec decode (bs:varint) (x:erased UInt64.t) : y:UInt64.t{(requires bs == encode(x)) (ensures y == x)}
   = 0
